\documentclass[twocolumn,draft]{article}
\usepackage{savetrees}
% a more conservative option:
% \documentclass[]{article}
% \usepackage{fullpage}

\usepackage[utf8]{inputenc}
\usepackage[T1]{fontenc}
\usepackage{microtype}

\usepackage{amssymb}
\usepackage{amsfonts}
\usepackage{amsmath}
\usepackage{amsthm}

\usepackage{todonotes}
\usepackage{graphicx}
\usepackage{showlabels}

\usepackage[english]{babel}
\usepackage{blindtext}
% \Blindtext to use.

\RequirePackage[l2tabu, orthodox]{nag}
\usepackage[all,warning]{onlyamsmath}

\usepackage{hyperref}

% blue text for questions
\newcommand{\bt}[1]{\textcolor{blue}{#1}}

\title{MA 341, 4/5/17}
\author{John M. Lynch\footnote{Undergraduate ECE/Physics, NCSU, Raleigh, NC 27705. E-Mail: \texttt{jmlynch3@ncsu.edu}}}
\date{\today}

\begin{document}
  \maketitle
  
  \section*{Variation of Parameters}
  
  \begin{equation}
  	\frac{dx}{dt} = Ax + \rho(t)
  \end{equation}
  
  elaboration:
  
  \begin{align*}
  	\frac{dx}{dt} = Ax + \rho(t), \\
	A\in\Re^{n\times n}, \\
	x = \begin{bmatrix}
		x_{1} \\
		\vdots \\
		x_{n}
	\end{bmatrix}, \\
	\rho(t) = \begin{bmatrix}
				\rho_{1}(t) \\
				\vdots \\
				\rho_{n}(t)
			  \end{bmatrix}
  \end{align*}
  
  then
  
  \begin{equation}
  	\frac{dx}{dt} = Ax
  \end{equation}
  
  \subsection*{1) Find fundamental matrix X(t)} For $X(t)$, a fundamental matrix that solves
  
  \begin{align}
  	\frac{dX}{dt} &= AX \\
	(\frac{dX}{dt} - AX)C &= 0
  \end{align}
  
  then
  
  \begin{equation}
  	x(t) = X(t)C \text{(general solution)}
  \end{equation}
  
  where
  
  \begin{equation*}
  	C = \begin{bmatrix}
			C_{1} \\
			\vdots \\
			C_{n}
  		\end{bmatrix}
  \end{equation*}
  
  Find solutions of (1) in the form of
  
  \begin{equation*}
  	x(t) = X(t)\cdot C(t), C(t) = \begin{bmatrix}
  									C_{1}(t) \\
									\vdots \\
									C_{n}(t)
  								  \end{bmatrix}
  \end{equation*}
  
  substitute in:
  
  \begin{equation*}
  	\frac{dx}{dt} = \boxed{\frac{dX}{dt} \cdot C} + X\cdot \frac{dC}{dt} = \boxed{AXC} + \rho(t)
  \end{equation*}
  
  which leaves
  
 \subsection*{2) Find $X^{-1}$}
 
 \subsection*{3) Find $C(t)$}
  \begin{align*}
  	\frac{dC}{dt} &= \rho(t) \\
	\frac{dC}{dt} &= X^{-1}(t)\rho(t) \\
	C(t) &= \int X^{-1}(t)\rho(t)dt
  \end{align*}
  
  so you have your coefficient column vector $C(t)$.
  
  \subsection*{4) General Solution}
  
  \begin{equation}
  	x(t) = X(t) \cdot C(t)
  \end{equation}
  
  % EMPTY COLUMN
  \newpage
  
  \section*{EXAMPLE}
  
  \begin{equation}
  	A = \begin{bmatrix}
	0 & 1 \\
	-1 & 0
  	\end{bmatrix}
  \end{equation}
  
  \begin{equation}
  	\rho(t) = \begin{bmatrix}
	8\sin{(t)} \\
	0
  	\end{bmatrix}
  \end{equation}
  
  \subsection*{1)}
  
  \begin{align*}
  	\frac{dx}{dt} &= Ax \\
	det(A-rI) &= 0 \\
	det(\begin{bmatrix}
		-r & 1 \\
		-1 & -r
	\end{bmatrix}) &= r^{2} + 1 = 0 \\
	r \pm i
  \end{align*}
  
  Extract linear equations from matrix:
  
  \begin{equation}
  	\begin{bmatrix}
		-i & 1 \\
		-1 & -i
  	\end{bmatrix}
  \end{equation}
  
  \begin{align*}
	  -iu_{1} + u_{2} &= 0 \\
	  -u_{1} - iu_{2} &= 0
  \end{align*}
  
  If you don't drop an equation, one of your eigen values was wrong.
  
  Multiply first eqn by $i$:
  
  \begin{align*}
	  u_{1} + iu_{2} &= 0 \\
	  -u_{1} - iu_{2} &= 0
  \end{align*}
  
  and simplify:
  
  \begin{equation*}
	  \boxed{u_{1} + iu_{2} = 0}
  \end{equation*}
  
  \begin{align*}
 	u_{1} &= -is \\
	u_{2} &= s
  \end{align*}
  
  so
  
  % u = [-is \\ s] = s[-i \\ 1]
  
  and
  
  \begin{equation}
  	u = \begin{bmatrix}
  		0 \\ 1
  	\end{bmatrix} + i \begin{bmatrix}
  						-1 \\ 0
  					  \end{bmatrix}
  \end{equation}
  
  \subsection*{general solt'n}
  
  \begin{equation}
  	\Big(e^{\alpha t}\cos{(\beta t)}a - e^{\alpha t}\sin{(\beta t)}b\Big)C1 +
	\Big(e^{\alpha t}\cos{(\beta t)}a + e^{\alpha t}\sin{(\beta t)}b\Big)C2
  \end{equation}
  
  \begin{equation*}
  	x(t) = \Big(\cos{t \begin{bmatrix}
  						0 \\ 1
  						\end{bmatrix}}
				- \sin{t \begin{bmatrix}
							-1 \\ 0
							\end{bmatrix}}\Big)C_{1}
		 +
		 \Big(\sin{t \begin{bmatrix}
		   						0 \\ 1
		   						\end{bmatrix}}
		 				+ \cos{t \begin{bmatrix}
		 							-1 \\ 0
		 							\end{bmatrix}}\Big)C_{2}
  \end{equation*}
  
  \begin{equation*}
	x_{1}(t) = \begin{bmatrix}
					\sin{t} \\
					\cos{t}
				\end{bmatrix} ,
	x_{2}(t) = \begin{bmatrix}
					-\cos{t} \\
					\sin{t}
				\end{bmatrix}
  \end{equation*}
  
  \subsection*{construct fundamental matrix $X(t)$}
  
  \begin{equation}
  	X(t) = \begin{bmatrix}
				\sin{t} & -\cos{t} \\
				cos{t} & \sin{t}
		  	\end{bmatrix}
  \end{equation}
  
  \subsection*{find $X^{-1}$}
  
  For 2 by 2,
  
  \begin{equation*}
  	A^{-1} = \frac{1}{ad-bc} \begin{bmatrix}
  								d & -b \\
								-c & a
  							 \end{bmatrix}
  \end{equation*}
  
  \begin{equation*}
  	X^{-1} = \frac{1}{1} \begin{bmatrix}
  							\sin{t} & \cos{t} \\
							-\cos{t} & \sin{t}
  						 \end{bmatrix}
  \end{equation*}
  
  \begin{equation*}
	\begin{bmatrix}
		\sin{t} & \cos{t} \\
		-\cos{t} & \sin{t}
	\end{bmatrix}
	\begin{bmatrix}
		8\sin{t} \\
		0
	\end{bmatrix}
	=
	\begin{bmatrix}
		8\sin^{2}{t} \\
		-8\sin{t}\cos{t}
	\end{bmatrix}
  \end{equation*}
  
  \subsection*{integrate to find $C(t)$}
  
  \begin{equation*}
  	\int
	\begin{bmatrix}
		8\sin^{2}{t} \\
		-8\sin{t}\cos{t}
	\end{bmatrix}
	dt =
	\begin{bmatrix}
		\int 8\sin^{2}{t} dt \\
		\int -8\sin{t}\cos{t} dt
	\end{bmatrix}
  \end{equation*}
  
  \subsection*{integrate (i)}
  
  Use $\sin^{2}{t}=\frac{1-\cos{2t}}{2}$ and $\cos^{2}{t} = \frac{1+\cos{2t}}{2}$
  
  \begin{equation*}
  	\int 8\sin^{2}{t} dt = \int 4 (1 - \cos{2t})dt = \int (4 - 4\cos{2t})dt = 4t - 2\sin{2t} + C_{1}
  \end{equation*}
  
  \subsection*{integrate (ii)}
  
  \begin{equation*}
  	\int -8 \sin{t}\cos{t}dt = 2\cos{2t} + C_{2}
  \end{equation*}
 
 \subsection*{integrate (net)}
 
 \begin{equation*}
 	C(t) =
	\begin{bmatrix}
		4t - 2\sin{2t} + C_{1} \\
		2\cos{2t} + C_{2}
	\end{bmatrix}
 \end{equation*}
 
 \subsection*{general solution}
 
 \[
 	x(t) = X(t)\cdot C(t)
 \]
 
 In sum:
 
 \begin{enumerate}
 	\item find $X(t)$
	\item find $X^{-1}$
	\item find $C(t)$
	\item gen solt'n
 \end{enumerate}
 
 \newpage
 
 \section*{special fundamental matrix}
 
 \[
 	\frac{dx}{dt} = Ax
 \]
 
 \[
 	\frac{dX}{dt} = AX \leftarrow m\times n\text{matrices}
 \]
 
 \[
 	x(t) = X(t)C
 \]
 
 special fundamental matrix: instead of generic $C$ vals in col, you see initial conditions:
 
 \[
 	x(t) = X(t) x(0)
 \]
 
 an easy way to incorporate initial conditions, and computing this special $X(t)$ from the
 generic $X(t)$ isn't even hard.
 
 start with $Y(t)$, then, special $X(t)$ can be found by
 
 \[
 	X(t) = Y(t)\Big(Y(0)\Big)^{-1}
 \]
 
\end{document}